Finish proving unique decomposition.
The main insight is that: the proof of unique decomposition basically
contains an algorithm to "construct" the unique decomposition:

forall e, (exists v, e = v) \/ (exists! M R e', e = meta_rplug M (rplug R e'))

Notice the quantifier `exists`. In Rocq, we prove `exists` by giving the witness,
and we can only give the witness if we can construct it.

Therefore, a better idea is to extract the decomposition as a separate function,
which is much easier to study; and is useful to state our other lemmas as well.

After obtaining the decomposition function, we prove unique decomposition by
"delegating" to this decomposing function. We just need to prove that, given
a redex, an evaluation context and a meta context, plugging them and decomposing
them is identity. The prove is by pure equational reasoning (!) and it much easier
to understand.

ctx-equiv-ixfree/lang_shift_reset.v
@@ -314,6 +314,13 @@ Proof.
   exact (ectx_comp_rctx2_correct E rctx_hole e).
 Qed.
 
+Lemma rctx_to_ectx_correct {V} (R : rctx V) (e : expr V) :
+  plug (rctx_to_ectx R) e = rplug R e.
+Proof.
+  unfold rctx_to_ectx.
+  exact (ectx_comp_rctx1_correct ectx_hole R e).
+Qed.
+
 Lemma plug_eq_val_inv {V} E e (v : val V) :
   plug E e = v →
   E = ectx_hole ∧ e = v.
@@ -586,6 +593,10 @@ Proof. auto. Qed.
 Definition meta_ectx_comp {V} (M1 M2 : meta_ectx V) : meta_ectx V :=
   M2 ++ M1.
 
+Lemma fold_unfold_meta_ectx_comp {V} (M1 M2 : meta_ectx V) :
+  meta_ectx_comp M1 M2 = M2 ++ M1.
+Proof. auto. Qed.
+
 Lemma meta_plug_eq_val_inv {V} (M : meta_ectx V) (e : expr V) (v : val V) :
   meta_plug M e = v →
   M = [] ∧ e = v.
@@ -655,6 +666,99 @@ Proof. auto_bind_comp. Qed.
 #[global] Instance Bind_meta_ectx : Bind meta_ectx.
 Proof. constructor. exact @meta_ectx_bind_id. exact @meta_ectx_bind_comp. Qed.
 
+(** Outside-in meta context *)
+
+Definition meta_rctx V := list (rctx V).
+
+Fixpoint meta_rplug {V} (M : meta_rctx V) (e : expr V) : expr V :=
+  match M with
+  | [] => e
+  | R :: M => rplug R (e_reset (meta_rplug M e))
+  end.
+
+Definition meta_rctx_comp {V} : meta_rctx V → meta_rctx V → meta_rctx V :=
+  app.
+
+Lemma fold_unfold_meta_rctx_comp {V} (M1 M2 : meta_rctx V) :
+  meta_rctx_comp M1 M2 = M1 ++ M2.
+Proof. auto. Qed.
+
+Lemma meta_rplug_eq_val_inv {V} (M : meta_rctx V) (e : expr V) (v : val V) :
+  meta_rplug M e = v →
+  M = [] ∧ e = v.
+Proof.
+  intros H_eq.
+  destruct M as [| R M]; simpl in *.
+  - auto.
+  - apply rplug_eq_val_inv in H_eq as [_ H_absurd].
+    discriminate.
+Qed.
+
+Lemma meta_rctx_comp_correct {V} (M1 M2 : meta_rctx V) e :
+  meta_rplug (meta_rctx_comp M1 M2) e = meta_rplug M1 (meta_rplug M2 e).
+Proof.
+  induction M1 as [| R M1 IHM1].
+  - simpl. reflexivity.
+  - simpl. rewrite -> IHM1. reflexivity.
+Qed.
+
+Definition meta_ectx_to_meta_rctx {V} (M : meta_ectx V) : meta_rctx V :=
+  rev (map ectx_to_rctx M).
+
+Definition meta_rctx_to_meta_ectx {V} (M : meta_rctx V) : meta_ectx V :=
+  rev (map rctx_to_ectx M).
+
+Lemma meta_ectx_meta_rctx_bijection {V} (M : meta_ectx V) :
+  meta_rctx_to_meta_ectx (meta_ectx_to_meta_rctx M) = M.
+Proof.
+  unfold meta_ectx_to_meta_rctx, meta_rctx_to_meta_ectx.
+  rewrite -> map_rev.
+  rewrite -> rev_involutive.
+  rewrite -> map_map.
+  rewrite <- (List.map_id M) at 2.
+  apply map_ext. apply ectx_rctx_bijection.
+Qed.
+
+Lemma meta_rctx_meta_ectx_bijection {V} (M : meta_rctx V) :
+  meta_ectx_to_meta_rctx (meta_rctx_to_meta_ectx M) = M.
+Proof.
+  unfold meta_ectx_to_meta_rctx, meta_rctx_to_meta_ectx.
+  rewrite -> map_rev.
+  rewrite -> rev_involutive.
+  rewrite -> map_map.
+  rewrite <- (List.map_id M) at 2.
+  apply map_ext. apply rctx_ectx_bijection.
+Qed.
+
+Lemma meta_rctx_to_meta_ectx_correct {V} (M : meta_rctx V) (e : expr V) :
+  meta_plug (meta_rctx_to_meta_ectx M) e = meta_rplug M e.
+Proof.
+  unfold meta_rctx_to_meta_ectx.
+  induction M as [| R M IHM].
+  - simpl. reflexivity.
+  - simpl.
+    rewrite <- fold_unfold_meta_ectx_comp.
+    rewrite -> meta_ectx_comp_correct. simpl.
+    rewrite -> IHM.
+    rewrite -> rctx_to_ectx_correct.
+    reflexivity.
+Qed.
+
+Lemma meta_ectx_to_meta_rctx_correct {V} (M : meta_ectx V) (e : expr V) :
+  meta_rplug (meta_ectx_to_meta_rctx M) e = meta_plug M e.
+Proof.
+  revert e.
+  unfold meta_ectx_to_meta_rctx.
+  induction M as [| R M IHM]; intros e.
+  - simpl. reflexivity.
+  - simpl.
+    rewrite <- fold_unfold_meta_rctx_comp.
+    rewrite -> meta_rctx_comp_correct. simpl.
+    rewrite -> IHM.
+    rewrite -> ectx_to_rctx_correct.
+    reflexivity.
+Qed.
+
 (** Reduction *)
 
 Inductive base_step {V} : expr V → expr V → Prop :=
@@ -676,26 +780,6 @@ Inductive meta_contextual_step {V} : expr V → expr V → Prop :=
 | mcs_contextual (M : meta_ectx V) (e1 e2 : expr V) :
   contextual_step e1 e2 →
   meta_contextual_step (meta_plug M e1) (meta_plug M e2).
-
-(*
-Inductive contextual_step {V} : expr V → expr V → Prop :=
-| Ectx_beta_lambda MR R (e : expr (inc V)) (v : val V) :
-  contextual_step
-    (meta_plug MR (rplug R (e_app (v_lambda e) v)))
-    (meta_plug MR (rplug R (subst (Inc:=inc) e v)))
-| Ectx_shift MR R (e : expr (inc V)) :
-  contextual_step
-    (meta_plug MR (rplug R (e_shift e)))
-    (meta_plug MR (subst (Inc:=inc) e (v_cont R)))
-| Ectx_beta_cont MR R (R' : rctx V) (v : val V) :
-  contextual_step
-    (meta_plug MR (rplug R (e_app (v_cont R') v)))
-    (meta_plug MR (rplug R (e_reset (rplug R' v))))
-| Ectx_reset MR R (v : val V) :
-  contextual_step
-    (meta_plug MR (rplug R (e_reset v)))
-    (meta_plug MR (rplug R v)).
-*)
 
 Definition big_step {V} e (v : val V) :=
   rtc meta_contextual_step e v.
@@ -783,64 +867,149 @@ Lemma base_step_potential_redex {V} (e e' : expr V) :
   potential_redex e.
 Proof. inversion_clear 1; constructor. Qed.
 
-Lemma unique_rdecomposition {V} (R1 R2 : rctx V) e1 e2 :
-  potential_redex e1 →
-  potential_redex e2 →
-  rplug R1 e1 = rplug R2 e2 →
-  R1 = R2 ∧ e1 = e2.
+Fixpoint decompose {V} (e : expr V) : val V + (meta_rctx V * (rctx V * expr V)) :=
+  match e with
+  | e_val v => inl v
+  | e_app e1 e2 =>
+      inr
+        match decompose e1 with
+        | inl v1 =>
+            match decompose e2 with
+            | inl v2 => ([], (rctx_hole, e_app v1 v2))
+            | inr (M, p) =>
+                match M with
+                | [] => let (R, e2') := p in ([], (rctx_app2 v1 R, e2'))
+                | R :: M' => (rctx_app2 v1 R :: M', p)
+                end
+            end
+        | inr (M, p) =>
+            match M with
+            | [] => let (R, e1') := p in ([], (rctx_app1 R e2, e1'))
+            | R :: M' => (rctx_app1 R e2 :: M', p)
+            end
+        end
+  | e_shift e' => inr ([], (rctx_hole, e_shift e'))
+  | e_reset e' =>
+      inr
+        match decompose e' with
+        | inl v => ([], (rctx_hole, e_reset v))
+        | inr (M, p) => (rctx_hole :: M, p)
+        end
+  end.
+
+Lemma decompose_correct {V} (e : expr V) :
+  match decompose e with
+  | inl v => e_val v
+  | inr (M, (R, e')) => meta_rplug M (rplug R e')
+  end = e.
 Proof.
-  intros He1 He2.
-  revert R2.
-  induction R1; intros R2 Heq.
-  - destruct R2; simpl in *.
-    + auto.
-    + rewrite -> Heq in He1.
-      apply potential_redex_app_inv in He1 as (v1 & v2 & Hv1 & Hv2).
-      apply rplug_eq_val_inv in Hv1 as [_ ->].
-      contradict (not_potential_redex_val _ He2).
-    + rewrite -> Heq in He1.
-      apply potential_redex_app_inv in He1 as (v1 & v2 & Hv1 & Hv2).
-      apply rplug_eq_val_inv in Hv2 as [_ ->].
-      contradict (not_potential_redex_val _ He2).
-  - destruct R2; simpl in *.
-    + rewrite <- Heq in He2.
-      apply potential_redex_app_inv in He2 as (v1 & v2 & Hv1 & Hv2).
-      apply rplug_eq_val_inv in Hv1 as [_ ->].
-      contradict (not_potential_redex_val _ He1).
-    + injection Heq as Heq1 Heq2.
-      apply IHR1 in Heq1 as [Heq11 Heq12].
-      split; congruence.
-    + injection Heq as Heq1 Heq2.
-      apply rplug_eq_val_inv in Heq1 as [_ ->].
-      contradict (not_potential_redex_val _ He1).
-  - destruct R2; simpl in *.
-    + rewrite <- Heq in He2.
-      apply potential_redex_app_inv in He2 as (v1 & v2 & Hv1 & Hv2).
-      apply rplug_eq_val_inv in Hv2 as [_ ->].
-      contradict (not_potential_redex_val _ He1).
-    + injection Heq as Heq1 Heq2. symmetry in Heq1.
-      apply rplug_eq_val_inv in Heq1 as [_ ->].
-      contradict (not_potential_redex_val _ He2).
-    + injection Heq as Heq1 Heq2.
-      apply IHR1 in Heq2 as [Heq11 Heq12].
-      split; congruence.
+  induction e; simpl.
+  - reflexivity.
+  - destruct (decompose e1) as [v1 | (M & R & e1')].
+    + destruct (decompose e2) as [v2 | (M & R & e2')].
+      * simpl. congruence.
+      * destruct M as [| R' M'].
+        { simpl in *. congruence. }
+        { simpl in *. congruence. }
+    + destruct M as [| R' M'].
+      * simpl in *. congruence.
+      * simpl in *. congruence.
+  - reflexivity.
+  - destruct (decompose e) as [v | (M & R & e')].
+    + simpl in *. congruence.
+    + simpl in *. congruence.
 Qed.
 
-Lemma unique_decomposition {V} (E1 E2 : ectx V) e1 e2 :
+Lemma decompose_redex {V} (e : expr V) :
+  match decompose e with
+  | inl _ => True
+  | inr (_, (_, e')) => potential_redex e'
+  end.
+Proof.
+  induction e; simpl.
+  - exact I.
+  - destruct (decompose e1) as [v1 | (M & R & e1')].
+    + destruct (decompose e2) as [v2 | (M & R & e2')].
+      * simpl. constructor.
+      * destruct M as [| R' M'].
+        { exact IHe2. }
+        { exact IHe2. }
+    + destruct M as [| R' M'].
+      * exact IHe1.
+      * exact IHe1.
+  - constructor.
+  - destruct (decompose e) as [v | (M & R & e')].
+    + constructor.
+    + exact IHe.
+Qed.
+
+Lemma decompose_unique_nil {V} R (e : expr V) :
+  potential_redex e →
+  decompose (rplug R e) = inr ([], (R, e)).
+Proof.
+  intros He.
+  induction R as [| R IHR e' | v' R IHR]; simpl in *.
+  - inversion_clear He; simpl in *.
+    + reflexivity.
+    + reflexivity.
+    + reflexivity.
+  - rewrite -> IHR. reflexivity.
+  - rewrite -> IHR. reflexivity.
+Qed.
+
+Lemma decompose_unique_cons {V} R M p (e : expr V) :
+  decompose e = inr (M, p) →
+  decompose (rplug R (e_reset e)) = inr (R :: M, p).
+Proof.
+  intros He.
+  induction R as [| R IHR e' | v' R IHR]; simpl in *.
+  - rewrite -> He. reflexivity.
+  - rewrite -> IHR. reflexivity.
+  - rewrite -> IHR. reflexivity.
+Qed.
+
+Lemma decompose_unique {V} M R (e : expr V) :
+  potential_redex e →
+  decompose (meta_rplug M (rplug R e)) = inr (M, (R, e)).
+Proof.
+  intros He.
+  induction M.
+  - simpl. apply decompose_unique_nil. exact He.
+  - simpl. apply decompose_unique_cons. exact IHM.
+Qed.
+
+Lemma unique_rdecomposition {V} (M1 M2 : meta_rctx V) (R1 R2 : rctx V) e1 e2 :
   potential_redex e1 →
   potential_redex e2 →
-  plug E1 e1 = plug E2 e2 →
-  E1 = E2 ∧ e1 = e2.
+  meta_rplug M1 (rplug R1 e1) = meta_rplug M2 (rplug R2 e2) →
+  M1 = M2 ∧ R1 = R2 ∧ e1 = e2.
 Proof.
   intros He1 He2 Heq.
-  rewrite <- ectx_to_rctx_correct in Heq.
-  rewrite <- ectx_to_rctx_correct in Heq.
-  destruct (unique_rdecomposition _ _ _ _ He1 He2 Heq) as [Heq1 Heq2].
-  split.
-  - rewrite <- (ectx_rctx_bijection E1).
-    rewrite <- (ectx_rctx_bijection E2).
-    f_equal. exact Heq1.
-  - exact Heq2.
+  assert (H_decompose1 := decompose_unique M1 R1 e1 He1).
+  assert (H_decompose2 := decompose_unique M2 R2 e2 He2).
+  rewrite -> Heq in H_decompose1.
+  rewrite -> H_decompose1 in H_decompose2.
+  injection H_decompose2. auto.
+Qed.
+
+Lemma unique_decomposition {V}
+  (M1 M2 : meta_ectx V) (E1 E2 : ectx V) e1 e2 :
+  potential_redex e1 →
+  potential_redex e2 →
+  meta_plug M1 (plug E1 e1) = meta_plug M2 (plug E2 e2) →
+  M1 = M2 ∧ E1 = E2 ∧ e1 = e2.
+Proof.
+  intros He1 He2 Heq.
+  rewrite <- (ectx_rctx_bijection E1) in Heq |- *.
+  rewrite <- (ectx_rctx_bijection E2) in Heq |- *.
+  rewrite <- (meta_ectx_meta_rctx_bijection M1) in Heq |- *.
+  rewrite <- (meta_ectx_meta_rctx_bijection M2) in Heq |- *.
+  rewrite -> meta_rctx_to_meta_ectx_correct in Heq.
+  rewrite -> meta_rctx_to_meta_ectx_correct in Heq.
+  rewrite -> rctx_to_ectx_correct in Heq.
+  rewrite -> rctx_to_ectx_correct in Heq.
+  apply unique_rdecomposition in Heq as (HM & HE & He); auto.
+  repeat split; congruence.
 Qed.
 
 Lemma contextual_step_is_deterministic {V} (e1 e2 e3 : expr V) :
@@ -1782,8 +1951,6 @@ Proof.
     - apply compat_ectx_app1. exact IHE. apply fundamental_property_e.
     - apply compat_ectx_app2. apply fundamental_property_v. exact IHE. }
 Qed.
-
-Print Assumptions fundamental_property_v.
 
 (** General program contexts *)
 Inductive ctx : Set → Type :=
